
\begin{equation*}

\Delta G_{R \rightarrow A} = \Delta G_{A}^f - \Delta G^f_{R}
\\
\Delta G_{HA^+ \rightarrow HR^+} = \Delta G_{HR^+}^f - \Delta G_{HA^+}^f
\\
0 = \Delta G_{A \rightarrow HA^+} + \Delta G_{HA^+ \rightarrow HR^+} - \Delta G_{R \rightarrow RH^+}  + \Delta G_{R \rightarrow A}
\\
\Delta G_{A \rightarrow HA^+} = \Delta G_{R \rightarrow HR^+} - \Delta G_{R \rightarrow A} - \Delta G_{HA^+ \rightarrow HR^+}
\\
\Delta G_{A \rightarrow HA^+} = \Delta G_{R \rightarrow HR^+} - \left ( \Delta G_A^f  - \Delta G_R^f \right ) - \left ( \Delta G_{HR^+}^f - \Delta G_{HA^+}^f \right )
\\
\Delta G_{A \rightarrow HA^+} = \Delta G_{R \rightarrow HR^+} + \left ( \Delta G_R^f - \Delta G_A^f \right ) + \left ( \Delta G_{HA^+}^f - \Delta G_{HR^+}^f \right )
\\
\Delta G_{A \rightarrow HA^+} = \Delta G_{R \rightarrow HR^+} + (\Delta G_R^f - \Delta G_{HR^+}^f) + \left ( \Delta G_{HA^+}^f - \Delta G_A^f \right )
\\
-PA_A = -PA_R^M + PA_R^C - PA_A^C
\\
PA_A = PA_A^C + \left ( PA_R^M - PA_R^C \right ) = PA_A^C + PA_R^{er}

\end{equation*}
